Progress on Lib.Buffer

lib/Lib.Buffer.fsti
@@ -15,19 +15,30 @@ module HS = FStar.HyperStack
 module Seq = Lib.Sequence
 module ByteSeq = Lib.ByteSequence
 
+
 #set-options "--z3rlimit 15"
 
 inline_for_extraction noextract
 let v = size_v
 
+(** Definition of a mutable Buffer *)
 let buffer (a:Type0) = B.buffer a
 
-val length: #a:Type0 -> b:buffer a -> GTot (r:size_nat{r == B.length b})
+(** Definition of an immutable Buffer *)
+let ibuffer (a:Type0) = IB.ibuffer a
 
+(** Length of buffers *)
+val length: #a:Type0 -> b:buffer a -> GTot (r:size_nat{r == B.length b})
+val ilength: #a:Type0 -> b:ibuffer a -> GTot (r:size_nat{r == IB.length b})
+
+(** Definition of fixed length mutable and immutable Buffers *)
 let lbuffer (a:Type0) (len:size_nat) = b:buffer a {length b == len}
-let libuffer (a:Type0) (len:size_nat) = b:IB.ibuffer a{IB.length b == len}
+let ilbuffer (a:Type0) (len:size_nat) = b:IB.ibuffer a{IB.length b == len}
+
+(** Alias for mutable buffer of bytes *)
 let lbytes len = lbuffer uint8 len
 
+(** Ghost view of a subset of a mutable Buffer *)
 let gsub
     (#a:Type0)
     (#len:size_nat)
@@ -38,7 +49,7 @@ let gsub
  =
   B.gsub b (size_to_UInt32 start) (size_to_UInt32 n)
 
-
+(** Subset of a mutable Buffer *)
 inline_for_extraction
 val sub:
     #a:Type0
@@ -46,140 +57,153 @@ val sub:
   -> #olen:size_nat
   -> b:lbuffer a len
   -> start:size_t
-  -> n:size_t{v start + v n <= len /\ v n == olen}
-  -> Stack (lbuffer a olen)
+  -> n:size_t{v start + v n <= len /\ v n == olen} ->
+  Stack (lbuffer a olen)
     (requires fun h0 -> B.live h0 b)
     (ensures  fun h0 r h1 ->
       h0 == h1 /\ r == B.gsub b (size_to_UInt32 start) (size_to_UInt32 n) /\
       B.as_seq h1 r == Seq.sub #a #len (B.as_seq h0 b) (v start) (v n))
 
+(** Subset of an immutable Buffer *)
 inline_for_extraction
 val isub:
     #a:Type0
   -> #len:size_nat
   -> #olen:size_nat
-  -> b:libuffer a len
+  -> b:ilbuffer a len
   -> start:size_t
-  -> n:size_t{v start + v n <= len /\ v n == olen}
-  -> Stack (libuffer a olen)
+  -> n:size_t{v start + v n <= len /\ v n == olen} ->
+  Stack (ilbuffer a olen)
     (requires fun h0 -> IB.live h0 b)
     (ensures  fun h0 r h1 ->
       h0 == h1 /\ r == IB.igsub b (size_to_UInt32 start) (size_to_UInt32 n) /\
       IB.as_seq h1 r == Seq.sub #a #len (IB.as_seq h0 b) (v start) (v n))
 
+(** Access a specific value in an mutable Buffer *)
 inline_for_extraction
 val index:
     #a:Type0
   -> #len:size_nat
   -> b:lbuffer a len
-  -> i:size_t{v i < len}
-  -> Stack a
+  -> i:size_t{v i < len} ->
+  Stack a
     (requires fun h0 -> B.live h0 b)
     (ensures  fun h0 r h1 -> h0 == h1 /\
       r == Seq.index #a #len (B.as_seq h1 b) (v i))
 
+(** Access a specific value in an immutable Buffer *)
 inline_for_extraction
 val iindex:
     #a:Type0
   -> #len:size_nat
-  -> b:libuffer a len
-  -> i:size_t{v i < len}
-  -> Stack a
+  -> b:ilbuffer a len
+  -> i:size_t{v i < len} ->
+  Stack a
     (requires fun h0 -> B.live h0 b)
     (ensures  fun h0 r h1 -> h0 == h1 /\
       r == Seq.index #a #len (IB.as_seq h1 b) (v i))
 
+(** Update a specific value in a mutable Buffer *)
 inline_for_extraction
 val upd:
     #a:Type0
   -> #len:size_nat{len > 0}
   -> b:lbuffer a len
   -> i:size_t{v i < len}
-  -> x:a
-  -> Stack unit
+  -> x:a ->
+  Stack unit
     (requires fun h0 -> B.live h0 b)
     (ensures  fun h0 _ h1 ->
       B.modifies (B.loc_buffer b) h0 h1 /\ B.live h1 b /\
       B.as_seq h1 b == Seq.upd #a #len (B.as_seq h0 b) (v i) x)
 
+(** Operator definition to update a mutable Buffer *)
 inline_for_extraction
 let op_Array_Assignment #a #len = upd #a #len
 
+(** Operator definition to access a mutable Buffer *)
 inline_for_extraction
 let op_Array_Access #a #len = index #a #len
 
+(** Access to the pure sequence-based value associated to an index of a Buffer  *)
 let bget (#a:Type0) (#len:size_nat) h (b:lbuffer a len) i = Seq.index #a #len (B.as_seq h b) i
+let ibget (#a:Type0) (#len:size_nat) h (b:ilbuffer a len) i = Seq.index #a #len (IB.as_seq h b) i
 
-unfold
-let ibget #a #n h (b:libuffer a n) i = Seq.index #_ #n (IB.as_seq h b) i
-
+(** Allocate a fixed-length mutable Buffer and initialize it to value [init] *)
 inline_for_extraction
 val create:
     #a:Type0
   -> #len:size_nat
   -> clen:size_t{v clen == len}
-  -> init:a
-  -> StackInline (lbuffer a len)
+  -> init:a ->
+  StackInline (lbuffer a len)
     (requires fun h0 -> len > 0)
     (ensures  fun h0 b h1 ->
       B.alloc_post_mem_common b h0 h1 (Seq.create len init) /\
       B.frameOf b = HS.get_tip h0)
 
+(** Allocate a fixed-length mutable Buffer based on an existing List *)
 inline_for_extraction noextract
 val createL:
     #a:Type0
-  -> init:list a{List.Tot.length init <= max_size_t}
-  -> StackInline (lbuffer a (normalize_term (List.Tot.length init)))
+  -> init:list a{List.Tot.length init <= max_size_t} ->
+  StackInline (lbuffer a (normalize_term (List.Tot.length init)))
     (requires fun h0 -> B.alloca_of_list_pre #a init)
     (ensures fun h0 b h1 ->
       B.alloc_post_mem_common b h0 h1 (Seq.of_list init) /\
       B.frameOf b = HS.get_tip h0)
 
+(** Recall the value of a top-level Buffer *)
+(* BB. Do we use this for mutable top-level buffers ? or should it be an ilbuffer *)
 inline_for_extraction
 val recall:
   #a:Type
   -> #len:size_nat
-  -> b:lbuffer a len
-  -> Stack unit
-  (requires fun _ -> B.recallable b)
-  (ensures  fun m0 _ m1 -> m0 == m1 /\ B.live m1 b)
+  -> b:lbuffer a len ->
+  Stack unit
+    (requires fun _ -> B.recallable b)
+    (ensures  fun m0 _ m1 -> m0 == m1 /\ B.live m1 b)
 
+(** Allocate a top-level fixed-length mutable Buffer and initialize it to value [init] *)
 inline_for_extraction noextract
 val createL_global:
     #a:Type0
-  -> init:list a{List.Tot.length init <= max_size_t}
-  -> ST (b:lbuffer a (normalize_term (List.Tot.length init)){
-    B.frameOf b == HyperStack.root /\ B.recallable b})
+  -> init:list a{List.Tot.length init <= max_size_t} ->
+  ST (b:lbuffer a (normalize_term (List.Tot.length init)){
+      B.frameOf b == HyperStack.root /\ B.recallable b})
     (requires fun h0 -> B.gcmalloc_of_list_pre #a HyperStack.root init)
     (ensures  fun h0 b h1 ->
       B.alloc_post_mem_common b h0 h1 (Seq.of_list init))
 
+(** Copy a mutable Buffer in another mutable Buffer *)
 inline_for_extraction
 val copy:
     #a:Type
   -> #len:size_nat
   -> o:lbuffer a len
   -> clen:size_t{v clen == len}
-  -> i:lbuffer a len
-  -> Stack unit
+  -> i:lbuffer a len ->
+  Stack unit
     (requires fun h0 -> B.live h0 o /\ B.live h0 i /\ B.disjoint i o)
     (ensures  fun h0 _ h1 ->
       B.live h1 o /\ B.live h1 i /\ B.modifies (B.loc_buffer o) h0 h1 /\
       B.as_seq h1 o == B.as_seq h0 i)
 
+(** Copy an immutable Buffer in a mutable Buffer *)
 inline_for_extraction
 val icopy:
     #a:Type
   -> #len:size_nat
   -> o:lbuffer a len
   -> clen:size_t{v clen == len}
-  -> i:libuffer a len
-  -> Stack unit
+  -> i:ilbuffer a len ->
+  Stack unit
     (requires fun h0 -> B.live h0 o /\ B.live h0 i /\ B.disjoint i o)
     (ensures  fun h0 _ h1 ->
       B.live h1 o /\ B.live h1 i /\ B.modifies (B.loc_buffer o) h0 h1 /\
       B.as_seq h1 o == B.as_seq h0 i)
 
+(** Copy a mutable Buffer in a part of another mutable Buffer *)
 inline_for_extraction
 val update_sub:
     #a:Type
@@ -187,12 +211,13 @@ val update_sub:
   -> dst:lbuffer a len
   -> start:size_t
   -> n:size_t{v start + v n <= len}
-  -> src:lbuffer a (size_v n)
-  -> Stack unit
+  -> src:lbuffer a (size_v n) ->
+  Stack unit
     (requires fun h -> B.live h dst /\ B.live h src /\ B.disjoint dst src)
     (ensures  fun h0 _ h1 -> B.live h1 dst /\ B.modifies (B.loc_buffer dst) h0 h1 /\
       B.as_seq h1 dst == Seq.update_sub #a #len (B.as_seq h0 dst) (v start) (v n) (B.as_seq h0 src))
 
+(** Copy an immutable Buffer in a part of a mutable Buffer *)
 inline_for_extraction
 val update_isub:
     #a:Type
@@ -200,12 +225,13 @@ val update_isub:
   -> dst:lbuffer a len
   -> start:size_t
   -> n:size_t{v start + v n <= len}
-  -> src:libuffer a (size_v n)
-  -> Stack unit
+  -> src:ilbuffer a (size_v n) ->
+  Stack unit
     (requires fun h -> B.live h dst /\ B.live h src /\ B.disjoint dst src)
     (ensures  fun h0 _ h1 -> B.live h1 dst /\ B.modifies (B.loc_buffer dst) h0 h1 /\
       B.as_seq h1 dst == Seq.update_sub #a #len (B.as_seq h0 dst) (v start) (v n) (B.as_seq h0 src))
 
+(** Update a part of a mutable Buffer in-place with the application of a function F on another Buffer *)
 inline_for_extraction
 val update_sub_f:
     #a:Type
@@ -218,8 +244,8 @@ val update_sub_f:
         (requires fun h -> B.live h b)
         (ensures  fun h0 _ h1 ->
 	  B.modifies (B.loc_buffer b) h0 h1 /\
-	  B.as_seq h1 b == spec h0))
-  -> Stack unit
+	  B.as_seq h1 b == spec h0)) ->
+  Stack unit
     (requires fun h -> B.live h buf)
     (ensures  fun h0 _ h1 -> B.modifies (B.loc_buffer buf) h0 h1 /\
       B.as_seq h1 buf == Seq.update_sub #a #len (B.as_seq h0 buf) (v start) (v n) (spec h0))
@@ -235,8 +261,8 @@ val loop_nospec:
   -> impl:
       (i:size_t{v i < v n} -> Stack unit
         (requires fun h -> B.modifies (B.loc_buffer buf) h0 h)
-        (ensures  fun _ _ h1 -> B.modifies (B.loc_buffer buf) h0 h1))
-  -> Stack unit
+        (ensures  fun _ _ h1 -> B.modifies (B.loc_buffer buf) h0 h1)) ->
+  Stack unit
     (requires fun h -> h0 == h /\ B.live h0 buf)
     (ensures  fun _ _ h1 -> B.modifies (B.loc_buffer buf) h0 h1)
 
@@ -253,6 +279,7 @@ val loop_nospec:
 * - [spec] a specification of how the body of the loop modifies the state
 * - [impl] the body of the loop as a Stack function
 *)
+
 inline_for_extraction noextract
 let loop_inv
     (h0:mem)
@@ -265,7 +292,7 @@ let loop_inv
     (spec:(mem -> GTot (i:size_nat{i < v n} -> a_spec i -> a_spec (i + 1))))
     (i:size_nat{i <= v n})
     (h:mem) : Type0
- =
+  =
   B.modifies (footprint i) h0 h /\
   refl h i == Seq.repeat i a_spec (spec h0) (refl h0 0)
 
@@ -281,40 +308,43 @@ val loop:
   -> spec:(mem -> GTot (i:size_nat{i < v n} -> a_spec i -> a_spec (i + 1)))
   -> impl:(i:size_t{v i < v n} -> Stack unit
      (requires loop_inv h0 n a_spec a_impl acc refl footprint spec (v i))
-     (ensures  fun _ _ -> loop_inv h0 n a_spec a_impl acc refl footprint spec (v i + 1)))
-  -> Stack unit
+     (ensures  fun _ _ -> loop_inv h0 n a_spec a_impl acc refl footprint spec (v i + 1))) ->
+  Stack unit
     (requires fun h -> h0 == h)
     (ensures  fun _ _ -> loop_inv h0 n a_spec a_impl acc refl footprint spec (v n))
 
+(** Invariant for Loop1: modifies only one Buffer *)
 inline_for_extraction noextract
 let loop1_inv
     (h0:mem)
     (n:size_t)
     (b: Type)
     (blen: size_nat)
-    (acc:lbuffer b blen)
+    (write:lbuffer b blen)
     (spec:(mem -> GTot (i:size_nat{i < v n} -> Seq.lseq b blen -> Seq.lseq b blen)))
     (i:size_nat{i <= v n})
     (h:mem) : Type0
  =
-  B.modifies (B.loc_buffer acc) h0 h /\
-  B.as_seq h acc == Seq.repeati i (spec h0) (B.as_seq h0 acc)
+  B.modifies (B.loc_buffer write) h0 h /\
+  B.as_seq h write == Seq.repeati i (spec h0) (B.as_seq h0 write)
 
+(** Loop which modifies a single buffer [write] *)
 inline_for_extraction noextract
 val loop1:
     #b:Type
   -> #blen:size_nat
   -> h0:mem
   -> n:size_t
-  -> acc:lbuffer b blen
+  -> write:lbuffer b blen
   -> spec:(mem -> GTot (i:size_nat{i < v n} -> Seq.lseq b blen -> Seq.lseq b blen))
   -> impl:(i:size_t{v i < v n} -> Stack unit
-     (requires loop1_inv h0 n b blen acc spec (v i))
-     (ensures  fun _ _ -> loop1_inv h0 n b blen acc spec (v i + 1)))
-  -> Stack unit
+     (requires loop1_inv h0 n b blen write spec (v i))
+     (ensures  fun _ _ -> loop1_inv h0 n b blen write spec (v i + 1))) ->
+  Stack unit
     (requires fun h -> h0 == h)
-    (ensures  fun _ _ -> loop1_inv h0 n b blen acc spec (v n))
+    (ensures  fun _ _ -> loop1_inv h0 n b blen write spec (v n))
 
+(** Invariant for Loop2: modifies two Buffers *)
 inline_for_extraction noextract
 let loop2_inv
     (#b0:Type)
@@ -323,18 +353,19 @@ let loop2_inv
     (#blen1:size_nat)
     (h0:mem)
     (n:size_t)
-    (acc0:lbuffer b0 blen0)
-    (acc1:lbuffer b1 blen1)
+    (write0:lbuffer b0 blen0)
+    (write1:lbuffer b1 blen1)
     (spec:(mem -> GTot (i:size_nat{i < v n}
                -> tuple2 (Seq.lseq b0 blen0) (Seq.lseq b1 blen1)
                -> tuple2 (Seq.lseq b0 blen0) (Seq.lseq b1 blen1))))
     (i:size_nat{i <= v n})
     (h:mem) : Type0
  =
-  B.modifies (B.loc_union (B.loc_buffer acc0) (B.loc_buffer acc1)) h0 h /\
-  (let s0, s1 = Seq.repeati i (spec h0) (B.as_seq h0 acc0, B.as_seq h0 acc1) in
-  B.as_seq h acc0 == s0 /\ B.as_seq h acc1 == s1)
+  B.modifies (B.loc_union (B.loc_buffer write0) (B.loc_buffer write1)) h0 h /\
+  (let s0, s1 = Seq.repeati i (spec h0) (B.as_seq h0 write0, B.as_seq h0 write1) in
+  B.as_seq h write0 == s0 /\ B.as_seq h write1 == s1)
 
+(** Loop which modifies two buffers [write0] and [write1] *)
 inline_for_extraction noextract
 val loop2:
      #b0:Type
@@ -343,30 +374,31 @@ val loop2:
   -> #blen1:size_nat
   -> h0:mem
   -> n:size_t
-  -> acc0:lbuffer b0 blen0
-  -> acc1:lbuffer b1 blen1
+  -> write0:lbuffer b0 blen0
+  -> write1:lbuffer b1 blen1
   -> spec:(mem -> GTot (i:size_nat{i < v n}
                -> tuple2 (Seq.lseq b0 blen0) (Seq.lseq b1 blen1)
                -> tuple2 (Seq.lseq b0 blen0) (Seq.lseq b1 blen1)))
   -> impl:(i:size_t{v i < v n} -> Stack unit
-    (requires loop2_inv #b0 #blen0 #b1 #blen1 h0 n acc0 acc1 spec (v i))
-    (ensures  fun _ _  -> loop2_inv #b0 #blen0 #b1 #blen1 h0 n acc0 acc1 spec (v i + 1)))
-  -> Stack unit
+      (requires loop2_inv #b0 #blen0 #b1 #blen1 h0 n write0 write1 spec (v i))
+      (ensures  fun _ _  -> loop2_inv #b0 #blen0 #b1 #blen1 h0 n write0 write1 spec (v i + 1))) ->
+  Stack unit
     (requires fun h -> h0 == h)
-    (ensures  fun _ _  -> loop2_inv #b0 #blen0 #b1 #blen1 h0 n acc0 acc1 spec (v n))
+    (ensures  fun _ _  -> loop2_inv #b0 #blen0 #b1 #blen1 h0 n write0 write1 spec (v n))
 
 (** Compares two byte buffers of equal length returning a bool *)
 inline_for_extraction
 val lbytes_eq:
     #len:size_t
   -> a:lbuffer uint8 (v len)
-  -> b:lbuffer uint8 (v len)
-  -> Stack bool
+  -> b:lbuffer uint8 (v len) ->
+  Stack bool
     (requires fun h -> B.live h a /\ B.live h b)
     (ensures  fun h0 r h1 ->
       B.modifies B.loc_none h0 h1 /\
       r == Seq.lbytes_eq #(v len) (B.as_seq h0 a) (B.as_seq h0 b))
 
+(** Allocates a mutable Buffer, perform computations [impl] and securely delete the allocated buffer *)
 inline_for_extraction
 val alloc:
     #a:Type0
@@ -379,8 +411,7 @@ val alloc:
   -> init:a
   -> write:lbuffer w wlen
   -> spec:(h:mem -> GTot(r:b -> Seq.lseq w wlen -> Type))
-  -> impl:(buf:lbuffer a len ->
-    Stack b
+  -> impl:(buf:lbuffer a len -> Stack b
       (requires (fun h -> B.modifies (B.loc_buffer buf) h0 h /\ B.live h0 write))
       (ensures (fun h r h' -> B.modifies (B.loc_union (B.loc_buffer buf) (B.loc_buffer write)) h h' /\
 			                  spec h0 r (B.as_seq h' write)))) ->
@@ -389,11 +420,12 @@ val alloc:
     (ensures (fun h0 r h1 -> B.modifies (B.loc_buffer write) h0 h1 /\
 		                    spec h0 r (B.as_seq h1 write)))
 
-// TODO: used in tests; move to a different module
+(** Print and compare two buffers securely *)
+(* BB. TODO: used in tests; move to Lib.Print *)
 val print_compare_display:
     len:size_t
   -> lbuffer uint8 (size_v len)
-  -> lbuffer uint8 (size_v len)
-  -> Stack unit
+  -> lbuffer uint8 (size_v len) ->
+  Stack unit
     (requires fun h -> True)
     (ensures fun h0 _ h1 -> h0 == h1)
